making the constructor changes and fraction changes as in simpleCell to doubleCount1 and share1

doubleCount1.bpl
@@ -1,35 +1,46 @@
 //type Ref represents object references
 type Ref;
 type PredicateTypes;
-type FractionType = [Ref, PredicateTypes] int;
+type FractionType = [Ref] int;
 type PackedType = [Ref, PredicateTypes] bool;
 var packed: PackedType;
-var frac: FractionType;
+var fracOKP: FractionType;
 const null: Ref;
 
 var val: [Ref]int;
 var dbl: [Ref]int;
 
-const unique okP: PredicateTypes;
+const unique OKP: PredicateTypes;
 
-procedure PackOK(this:Ref);
-requires (dbl[this]==val[this]*2);
+//Constructor for DoubleCount that ensures OK.
+//Might need to add a ConstructDoubleCount for the default constructor.
+procedure ConstructDoubleCount0(this: Ref, v: int, d: int);
+	ensures (val[this] == v) && 
+		(dbl[this] == d) && 
+		(packed[this, OKP]) && 
+		(fracOKP[this] >= 100);
 
-procedure UnpackOK(this:Ref);
-requires packed[this, okP];
-ensures (dbl[this]==val[this]*2);
+procedure PackOk(this:Ref);
+	requires (packed[this, OKP] == false) && 
+		(dbl[this]==val[this]*2);
+
+procedure UnpackOk(this:Ref);
+	requires packed[this, OKP] &&
+		(fracOKP[this] > 0);
+	ensures (dbl[this]==val[this]*2);
 
 
 procedure increment(this: Ref)
-modifies val, dbl, packed, frac;
-requires packed[this, okP]  && (frac[this, okP] > 0);
-ensures  packed[this, okP] && (frac[this, okP] > 0);
+	modifies val, dbl, packed, fracOKP;
+	requires packed[this, OKP]  && 
+		(fracOKP[this] > 0);
+	ensures  packed[this, OKP] && 
+		(fracOKP[this] > 0);
 {
-call UnpackOK(this);
-packed[this, okP]:=false;
-val[this]:= val[this]+1;
-dbl[this]:= dbl[this]+2;
-call PackOK(this);
-packed[this, okP]:=true;
+	call UnpackOk(this);
+	packed[this, OKP]:=false;
+	val[this]:= val[this]+1;
+	dbl[this]:= dbl[this]+2;
+	call PackOk(this);
+	packed[this, OKP]:=true;
 }
-
