share1.bpl
@@ -1,4 +1,4 @@
-//class DoubleCount
+//type Ref represents object references
 type Ref;
 type PredicateTypes;
 type FractionType = [Ref] int;
@@ -9,28 +9,42 @@ const null: Ref;
 
 var val: [Ref]int;
 var dbl: [Ref]int;
+
 const unique OKP: PredicateTypes;
 
-procedure PackOK(this:Ref);
-requires (dbl[this]==2*val[this]);
+//Constructor for DoubleCount that ensures OK.
+//Might need to add a ConstructDoubleCount for the default constructor.
+procedure ConstructDoubleCount0(this: Ref, v: int, d: int);
+	ensures (val[this] == v) && 
+		(dbl[this] == d) && 
+		(packed[this, OKP]) && 
+		(fracOKP[this] >= 100);
 
-procedure UnpackOK(this:Ref);
-requires packed[this, OKP];
-ensures (dbl[this]==2*val[this]);
+procedure PackOk(this:Ref);
+	requires (packed[this, OKP] == false) && 
+		(dbl[this]==val[this]*2);
 
-procedure increment(this:Ref)
-modifies val, dbl, packed;
-requires packed[this,OKP] && (fracOKP[this] > 0);
-ensures packed[this,OKP] && (fracOKP[this] > 0);
+procedure UnpackOk(this:Ref);
+	requires packed[this, OKP] &&
+		(fracOKP[this] > 0);
+	ensures (dbl[this]==val[this]*2);
+
+
+procedure increment(this: Ref)
+	modifies val, dbl, packed, fracOKP;
+	requires packed[this, OKP]  && 
+		(fracOKP[this] > 0);
+	ensures  packed[this, OKP] && 
+		(fracOKP[this] > 0);
 {
-call UnpackOK(this);
-packed[this, OKP]:=false;
-val[this]:=val[this]+1;
-dbl[this]:=dbl[this]+2;
-call PackOK(this);
-packed[this, OKP]:=true;
+	call UnpackOk(this);
+	packed[this, OKP]:=false;
+	val[this]:= val[this]+1;
+	dbl[this]:= dbl[this]+2;
+	call PackOk(this);
+	packed[this, OKP]:=true;
 }
- 
+
 //----------------------------------
 //class Share
 
@@ -39,63 +53,68 @@ var fracShareCountP: FractionType;
 
 const unique ShareCountP: PredicateTypes;
 
-//constructor for Share
-procedure ConstructShare(this:Ref, dc_:Ref);
-ensures dc[this] == dc_;
+//Constructor for Share
+//that packs to ShareCount
+procedure ConstructShare0(this:Ref, dc_:Ref);
+	ensures (dc[this] == dc_) &&
+		(packed[this, ShareCountP]) && 
+		(fracShareCountP[this] >= 100);
 
 procedure PackShareCount(this:Ref);
-requires (packed[dc[this], OKP] && (fracOKP[dc[this]] > 0));
+	requires (packed[dc[this], OKP] && 
+		(fracOKP[dc[this]] > 0));
 
 procedure UnpackShareCount(this:Ref);
-requires packed[this, ShareCountP];
-ensures (packed[dc[this], OKP] && (fracOKP[dc[this]] > 0));
+	requires packed[this, ShareCountP];
+	ensures (packed[dc[this], OKP] && 
+		(fracOKP[dc[this]] > 0));
 
 procedure touch(this: Ref)
-modifies val, dbl, packed;
-requires packed[this, ShareCountP] && (fracShareCountP[this] > 0);
-ensures packed[this, ShareCountP] && (fracShareCountP[this] > 0);
-//the way we automatically write this "free ensures" is described in point 4
-//in my email
-free ensures (forall x : Ref, y : PredicateTypes :: 
-(
-!((x==this) && (y==ShareCountP))
-==> (packed[x,y]==old(packed[x,y]))
-)
-);
+	modifies val, dbl, packed, fracOKP;
+	requires packed[this, ShareCountP] && 
+		(fracShareCountP[this] > 0);
+	ensures packed[this, ShareCountP] &&
+		(fracShareCountP[this] > 0);
+	//The way we automatically write this "free ensures" is described in point 4
+	//in my email.
+	free ensures (forall x : Ref, y : PredicateTypes :: 
+		(
+		!((x==this) && (y==ShareCountP))
+		==> (packed[x,y]==old(packed[x,y]))
+		)
+	);
 {
-call UnpackShareCount(this);
-packed[this, ShareCountP]:=false;
+	call UnpackShareCount(this);
+	packed[this, ShareCountP]:=false;
 
-assert (fracShareCountP[this] > 0);
-call increment(dc[this]) ;
-assert (fracShareCountP[this] > 0);
-call PackShareCount(this);
-packed[this, ShareCountP]:=true;
+	assert (fracShareCountP[this] > 0);
+	call increment(dc[this]) ;
+	assert (fracShareCountP[this] > 0);
+	call PackShareCount(this);
+	packed[this, ShareCountP]:=true;
 }
 
 procedure main()
-//need to add absolutely all global variables 
-//that are being modified, by this method,
-//or transitively by all methods that are called in 
-//this procedure
-modifies val, dbl, packed;
+	//need to add absolutely all global variables 
+	//that are being modified, by this method,
+	//or transitively by all methods that are called in 
+	//this procedure
+	modifies val, dbl, packed, fracOKP;
 {
+	//dc0 also needs to be constructed
 var dc0 : Ref;
 var share1, share2 : Ref;
-//need to state that dc0 satisfies the OK predicate
-//this is the way we state the invariant for dc0
-assume packed[dc0, OKP];
+//Need to state that dc0 satisfies the OK predicate.
+//By calling the constructorwe state the invariant for dc0.
+call ConstructDoubleCount0(dc0, 2, 4);
 
 
-call ConstructShare(share1, dc0);
-//this assume is for the dc of share1,
-//to say that we put it in the OK predicate
-assume fracOKP[dc[share1]] > 0;
+//By calling this constructorfor share1,
+//we say that we put it in the Share predicate.
+call ConstructShare0(share1, dc0);
 
-call ConstructShare(share2, dc0);
-//this assume is for the dc of share2,
-//to say that we put it in the OK predicate
-assume fracOKP[dc[share2]] > 0;
+
+call ConstructShare0(share2, dc0);
 
 
 //the 3 lines below are for creating the
@@ -103,16 +122,14 @@ assume fracOKP[dc[share2]] > 0;
 //share1@k ShareCount
 call PackShareCount(share1);
 packed[share1, ShareCountP] := true;
-assume (fracShareCountP[share1] > 0);
-
-call touch(share1);
 
 //the 3 lines below are for creating the
 //object proposition
 //share2@k ShareCount
 call PackShareCount(share2);
 packed[share2, ShareCountP] := true;
-assume (fracShareCountP[share2] > 0);
+
+call touch(share1);
 
 call touch(share2);
 }
